Clap/Lang/F/eq.lean
@@ -3,12 +3,12 @@ import Clap.Lang.FB.FB
 
 namespace Clap.Edsl.Lang.F
 
-def eq {p : ℕ} [Fact (p ≥ 2)] (a b : F p) : Edsl.CircuitStateM p (FB p) := do
+def eq {p : ℕ} [p.AtLeastTwo] (a b : F p) : Edsl.CircuitStateM p (FB p) := do
   Edsl.isZero (a - b)
 
 namespace eq
 
-lemma wellFormed {p : ℕ} [Fact (p ≥ 2)] (a b : F p):
+lemma wellFormed {p : ℕ} [p.AtLeastTwo] (a b : F p):
   (eq a b).wellFormed
 := by
   simp [eq]
@@ -16,36 +16,36 @@ lemma wellFormed {p : ℕ} [Fact (p ≥ 2)] (a b : F p):
 -- TODO represents
 def matchesBinaryBooleanFunctionWithSideEffects
   (p : ℕ)
-  [Fact (p ≥ 2)]
+  [p.AtLeastTwo]
   (spec_function : (ZMod p) → (ZMod p) → Bool)
   (function : (F p) → (F p) → Edsl.CircuitStateM p (FB p))
   (allocates : ℕ)
 : Prop :=
   ∀ (a b: F p) varStorePre numAlloc,
-  a.isValid (varStorePre.get?) →
-  b.isValid (varStorePre.get?) →
-  let a_eval := (a.eval varStorePre.get?).getD 0
-  let b_eval := (b.eval varStorePre.get?).getD 0
+  a.isValid varStorePre →
+  b.isValid varStorePre →
+  let a_eval := (a.eval varStorePre).getD 0
+  let b_eval := (b.eval varStorePre).getD 0
   let ⟨⟨result, circuit⟩, numAllocPostRun⟩ := ((function a b).run numAlloc)
     let ⟨numAllocPostEval, varStorePost, constraints⟩ := Edsl.CircuitState.eval
       circuit
       varStorePre
       numAlloc
-    result.eval varStorePost.get? = (FB.ofBool p (spec_function a_eval b_eval)).eval varStorePost.get? ∧
+    result.eval varStorePost = (FB.ofBool p (spec_function a_eval b_eval)).eval varStorePost ∧
     constraints = True ∧
     numAllocPostRun = numAlloc + allocates ∧
     numAllocPostRun = numAllocPostEval ∧
     ∀ i < numAlloc, varStorePost.get? i = varStorePre.get? i ∧
     let e := a-b
-    varStorePost.get? numAlloc = .some (if (e.eval varStorePre.get?) = .some 0 then 1 else 0)
+    varStorePost.get? numAlloc = .some (if (e.eval varStorePre) = .some 0 then 1 else 0)
 
-def spec (p : ℕ) [Fact (p ≥ 2)]: Prop := matchesBinaryBooleanFunctionWithSideEffects
+def spec (p : ℕ) [p.AtLeastTwo]: Prop := matchesBinaryBooleanFunctionWithSideEffects
   p
   (· == ·)
   F.eq
   (allocates := 1)
 
-lemma equiv (p : ℕ) [Fact (p ≥ 2)] :
+lemma equiv (p : ℕ) [p.AtLeastTwo] :
   spec p
 := by
   intro a b varStorePre numAlloc h_a_isValid h_b_isValid
