Clap/eDSLState/Monad.lean
@@ -294,6 +294,17 @@ lemma Vector_ofFnM_empty_state
     rewrite [this]; clear this
     simp [x, h]
 
+@[aesop safe forward, grind _=_]
+lemma mem_iff_isSome {p} {varStore : VarStore p} {x : FixedExp p} :
+  x ∈ varStore ↔ [varStore|x].isSome := by rfl
+
+lemma bind_eval {α} {a} {varStore : VarStore p} {f : ZMod p → Option α} (h : a ∈ varStore) :
+  [varStore|a] >>= f = f ([varStore|a].get h) := by aesop (add simp Option.bind)
+
+@[grind <=]
+lemma bind_eval' {α} {a} {varStore : VarStore p} {f : ZMod p → Option α} (h : a ∈ varStore) :
+  [varStore|a].bind f = f ([varStore|a].get h) := by aesop (add simp Option.bind)
+
 end
 
 end CircuitStateM
